Attempt2/Build/AndTree.dfy
@@ -1,0 +1,134 @@
+module Build.AndTree {
+
+  import opened Std.Wrappers
+
+  import opened Circ
+  import opened Eval
+  import opened ConservedSubcircuit
+  import opened Utils
+  import opened Entity
+  import opened MapFunction
+  import opened ConnectionEval
+  import opened Connection
+  import opened IslandBundle
+  import opened Subcircuit
+  import opened MapConnection
+  import opened CombineParallel
+  import opened CombineSeries
+
+  import opened AndBuilder
+  import opened IdentBuilder
+  import opened ConstBuilder
+
+  function AndTreeBehav(a: seq<bool>): bool
+  {
+    if |a| == 0 then
+      true
+    else if |a| == 1 then
+      a[0]
+    else if |a| == 2 then
+      a[0] && a[1]
+    else
+      var n := |a|;
+      var p := if n % 2 == 0 then n/2 else (n-1)/2;
+      AndTreeBehav(a[..p]) && AndTreeBehav(a[p..])
+  }
+
+  function AndTreeSF(n: nat, si: SI): (so: SO)
+    requires |si.inputs| == n
+    requires |si.state| == 0
+  {
+    SO([AndTreeBehav(si.inputs)], [])
+  }
+
+  ghost predicate MFReqs(n: nat, mf_a: MapFunction, mf_b: MapFunction, mf_and: MapFunction, mf_combined: MapFunction)
+  {
+    && n > 2
+    && var p := if n % 2 == 0 then n/2 else (n-1)/2;
+    && AndTreeMFValid(p, mf_a)
+    && AndTreeMFValid(n-p, mf_b)
+    && AndMFValid(mf_and)
+    && AndTreeMFValid(n, mf_combined)
+    && mf_a.NPs() !! mf_b.NPs()
+    && mf_combined.inputs == mf_a.inputs + mf_b.inputs
+    && mf_and.inputs == mf_and.inputs == mf_a.outputs + mf_b.outputs
+    && mf_combined.outputs == mf_and.outputs
+  }
+
+  ghost predicate AndTreeMFValid(n: nat, mf: MapFunction)
+  {
+    && mf.Valid()
+    && (|mf.inputs| == n)
+    && (|mf.state| == 0)
+    && (|mf.outputs| == 1)
+    && (forall si :: SIValid(si, mf.inputs, mf.state) ==> (
+      && mf.sf.requires(si)
+      && (mf.sf(si) == AndTreeSF(n, si))))
+  }
+  function {:vcs_split_on_every_assert} InsertAndTreeImpl(c: Circuit, n: nat): (r: (Circuit, Entity))
+    requires CircuitValid(c)
+    ensures CircuitValid(r.0)
+    ensures EntityValid(r.0, r.1)
+    ensures CircuitUnconnected(c, r.0)
+    ensures CircuitConserved(c, r.0)
+    ensures IsIsland(r.0, r.1.sc)
+    ensures r.0.NodeKind.Keys == c.NodeKind.Keys + r.1.sc
+    ensures c.NodeKind.Keys !! r.1.sc
+    ensures |r.1.mf.inputs| == n
+    decreases n
+  {
+    if n == 0 then
+      InsertConst(c, true)
+    else if n == 1 then
+      InsertIdent(c)
+    else if n == 2 then
+      InsertAnd(c)
+    else
+      var p := if n % 2 == 0 then n/2 else (n-1)/2;
+      var eb1 := IslandBundleFromCircuit(c);
+
+      // Insert the left part of the tree.
+      var (c1, e_left) := InsertAndTreeImpl(c, p);
+      assert c1.NodeKind.Keys == c.NodeKind.Keys + e_left.sc;
+      var (eb2, ref_left) := AddEntity(eb1, c1, e_left);
+      assert EntityValid(c1, e_left);
+      assert e_left == eb2.es[ref_left].value;
+
+      // Insert the right part of the tree.
+      var (c2, e_right) := InsertAndTreeImpl(c1, n-p);
+      assert c2.NodeKind.Keys == c1.NodeKind.Keys + e_right.sc;
+      var (eb3, ref_right) := AddEntity(eb2, c2, e_right);
+      assert EntityValid(c2, e_right);
+      assert EntityValid(c2, e_left) by {
+        reveal IslandBundleValid();
+      }
+      assert e_left == eb3.es[ref_left].value;
+      assert e_right == eb3.es[ref_right].value;
+
+      // Insert an 'and' connecting them.
+      var (c3, e_and) := InsertAnd(c2);
+      var (eb4, ref_and) := AddEntity(eb3, c3, e_and);
+
+      // Join the left and rights parts in parallel
+      assert CombineParallelEntitiesRequirements(eb4.c, e_left, e_right) by {
+        reveal IslandBundleValid();
+      }
+      var (eb5, ref_top) := IBCombineParallelEntities(eb4, ref_left, ref_right);
+      // Join the and on
+      var e_top := eb5.es[ref_top].value;
+      assert e_and == eb5.es[ref_and].value;
+      assert CombineSeriesEntitiesRequirements(eb5.c, e_top, e_and) by {
+        reveal IslandBundleValid();
+      }
+      var (eb6, ref_final) := IBCombineSeriesEntities(eb5, ref_top, ref_and);
+
+      var e_final := eb6.es[ref_final].value;
+
+      reveal IslandBundleValid();
+      assert CircuitUnconnected(c, eb6.c);
+      assert CircuitConserved(c, eb6.c);
+
+      (eb6.c, e_final)
+  }
+
+}
